compiler/backend/passes/proofs/thunk_to_envProofScript.sml
@@ -1,1095 +1,140 @@
 (*
-  Proof of correctness for the thunk_to_thunk compiler pass.
+  Proof of correctness for the thunk_to_env compiler pass.
  *)
 
 open HolKernel Parse boolLib bossLib term_tactic monadsyntax;
 open stringTheory optionTheory sumTheory pairTheory listTheory alistTheory
      pred_setTheory rich_listTheory thunkLang_primitivesTheory envLangTheory
      finite_mapTheory thunkLangTheory env_semanticsTheory thunk_semanticsTheory;
-open thunk_to_envTheory;
-open pure_miscTheory thunkLangPropsTheory;
+open thunk_to_envTheory thunk_to_env_1ProofTheory thunk_exp_ofTheory;
+open pure_miscTheory thunkLangPropsTheory thunk_cexpTheory;
 
 val _ = new_theory "thunk_to_envProof";
 
-val _ = set_grammar_ancestry ["pred_set", "rich_list", "envLang", "thunkLang",
-                              "thunk_to_env", "thunkLangProps", "env_semantics" ]
+val _ = set_grammar_ancestry ["thunk_to_envProof","thunk_exp_of"]
 
-val _ = numLib.prefer_num ();
-
-Inductive exp_rel:
-[exp_rel_Value:]
-  (∀env n v w.
-     ALOOKUP env n = SOME w ∧
-     v_rel v w ⇒
-       exp_rel env (Value v) (Var n)) ∧
-[exp_rel_Lit_Var:] (* Used in proof of interp_eq below *)
-  (∀env n s.
-     ALOOKUP env n = SOME (Atom s) ⇒
-       exp_rel env (Lit s) (Var n)) ∧
-[exp_rel_Unit_Var:] (* Used in proof of interp_eq below *)
-  (∀env n s.
-     ALOOKUP env n = SOME (Constructor s []) ⇒
-       exp_rel env (Cons s []) (Var n)) ∧
-[exp_rel_Var:]
-  (∀env n.
-     ALOOKUP env n = NONE ⇒
-       exp_rel env (Var n) (Var n)) ∧
-[exp_rel_App:]
-  (∀env x1 x2 y1 y2.
-     exp_rel env x1 x2 ∧
-     exp_rel env y1 y2 ⇒
-       exp_rel env (App x1 y1) (App x2 y2)) ∧
-[exp_rel_Lam:]
-  (∀env x y s.
-     exp_rel (FILTER (λ(n,x). n ≠ s) env) x y ⇒
-       exp_rel env (Lam s x) (Lam s y)) ∧
-[exp_rel_Let_NONE:]
-  (∀env x1 x2 y1 y2.
-     exp_rel env x1 x2 ∧
-     exp_rel env y1 y2 ⇒
-       exp_rel env (Let NONE x1 y1) (Let NONE x2 y2)) ∧
-[exp_rel_Let_SOME:]
-  (∀env x1 x2 y1 y2 s.
-     exp_rel env x1 x2 ∧
-     exp_rel (FILTER (λ(n,x). n ≠ s) env) y1 y2 ⇒
-       exp_rel env (Let (SOME s) x1 y1) (Let (SOME s) x2 y2)) ∧
-[exp_rel_If:]
-  (∀env x1 x2 y1 y2 z1 z2.
-     LIST_REL (exp_rel env) [x1;y1;z1] [x2;y2;z2] ⇒
-       exp_rel env (If x1 y1 z1) (If x2 y2 z2)) ∧
-[exp_rel_Prim:]
-  (∀env op xs ys.
-     LIST_REL (exp_rel env) xs ys ⇒
-       exp_rel env (Prim op xs) (Prim op ys)) ∧
-[exp_rel_Letrec:]
-  (∀env f g x y.
-     LIST_REL (λ(fn,b) (gn,c). fn = gn ∧
-                 exp_rel (FILTER (λ(n,x). ¬MEM n (MAP FST f)) env) b c)
-              (REVERSE f) g ∧
-     exp_rel (FILTER (λ(n,x). ¬MEM n (MAP FST f)) env) x y ⇒
-       exp_rel env (Letrec f x) (Letrec g y)) ∧
-[exp_rel_Delay:]
-  (∀env x y.
-     exp_rel env x y ⇒
-       exp_rel env (Delay x) (Delay y)) ∧
-[exp_rel_Box:]
-  (∀env x y.
-     exp_rel env x y ⇒
-       exp_rel env (Box x) (Box y)) ∧
-[exp_rel_Force:]
-  (∀env x y.
-     exp_rel env x y ⇒
-       exp_rel env (Force x) (Force y)) ∧
-[v_rel_Constructor:]
-  (∀s vs ws.
-     LIST_REL v_rel vs ws ⇒
-       v_rel (Constructor s vs) (Constructor s ws)) ∧
-[v_rel_Closure:]
-  (∀env s x y.
-     exp_rel env (Lam s x) (Lam s y) ⇒
-       v_rel (Closure s x) (Closure s env y)) ∧
-[v_rel_Recclosure:]
-  (∀env f g n.
-     LIST_REL (λ(fn,b) (gn,c). fn = gn ∧
-                 exp_rel (FILTER (λ(n,x). ¬MEM n (MAP FST f)) env) b c)
-              (REVERSE f) g ⇒
-       v_rel (Recclosure f n) (Recclosure g env n)) ∧
-[v_rel_Thunk_v:]
-  (∀v w.
-     v_rel v w ⇒
-       v_rel (Thunk (INL v)) (Thunk (INL w))) ∧
-[v_rel_Thunk_exp:]
-  (∀env x y.
-     exp_rel env x y ⇒
-       v_rel (Thunk (INR x)) (Thunk (INR (env, y)))) ∧
-[v_rel_Atom:]
-  (∀l.
-     v_rel (Atom l) (Atom l))
+Definition Lams_def:
+  Lams [] x = x ∧
+  Lams (y::ys) x = env_cexp$Lam y (Lams ys x)
 End
 
-Theorem v_rel_cases = CONJUNCT2 exp_rel_cases;
-
-Theorem exp_rel_def =
-  [ “exp_rel env (Value v) y”,
-    “exp_rel env (Var v) y”,
-    “exp_rel env (Prim op xs) y”,
-    “exp_rel env (App x y) z”,
-    “exp_rel env (Lam s x) y”,
-    “exp_rel env (Let NONE x y) z”,
-    “exp_rel env (Let (SOME s) x y) z”,
-    “exp_rel env (If x y z) w”,
-    “exp_rel env (Letrec f x) y”,
-    “exp_rel env (Delay x) y”,
-    “exp_rel env (Box x) y”,
-    “exp_rel env (Force x) y” ]
-  |> map (SIMP_CONV (srw_ss ()) [Once exp_rel_cases])
-  |> LIST_CONJ;
-
-Theorem v_rel_def =
-  [ “v_rel (Closure s x) z”,
-    “v_rel z (Closure s env x)”,
-    “v_rel (Recclosure s x) z”,
-    “v_rel z (Recclosure s funs x)”,
-    “v_rel (Constructor s x) z”,
-    “v_rel z (Constructor s x)”,
-    “v_rel (Atom s) z”,
-    “v_rel z (Atom s)”,
-    “v_rel (Thunk (INL s)) z”,
-    “v_rel z (Thunk (INL s))”,
-    “v_rel (Thunk (INR s)) z”,
-    “v_rel z (Thunk (INR (env, s)))” ]
-  |> map (SIMP_CONV (srw_ss ()) [Once v_rel_cases])
-  |> LIST_CONJ;
-
-Definition env_rel_def:
-  env_rel binds env =
-    LIST_REL (λ(f,v) (g,w). f = g ∧ v_rel v w) (REVERSE binds) env
+Definition Apps_def:
+  Apps x [] = x ∧
+  Apps x (y::ys) = Apps (env_cexp$App x y) ys
 End
 
-Theorem env_rel_OPTREL[local]:
-  env_rel binds env ⇒
-    ∀k. OPTREL v_rel (ALOOKUP (REVERSE binds) k) (ALOOKUP env k)
-Proof
-  rw [env_rel_def]
-  \\ ‘env = REVERSE (REVERSE env)’
-    by gs []
-  \\ pop_assum SUBST_ALL_TAC
-  \\ irule LIST_REL_OPTREL \\ gs []
-QED
-
-Theorem env_rel_MAP_FST[local]:
-  env_rel binds env ⇒
-    MAP FST (REVERSE binds) = MAP FST env
-Proof
-  rw [env_rel_def]
-  \\ irule LIST_EQ
-  \\ gvs [LIST_REL_EL_EQN, EL_MAP, EL_REVERSE, ELIM_UNCURRY]
-QED
-
-Theorem exp_rel_subst:
-  exp_rel (FILTER (λ(n,x). ¬MEM n (MAP FST binds)) env) x y ∧
-  env_rel binds extra ⇒
-    exp_rel (extra ++ env) (subst binds x) y
-Proof
-  ‘(∀env' x y.
-     exp_rel env' x y ⇒
-       ∀env binds extra.
-         env' = FILTER (λ(n,x). ¬MEM n (MAP FST binds)) env ∧
-         env_rel binds extra ⇒
-           exp_rel (extra ++ env) (subst binds x) y) ∧
-   (∀v w. v_rel v w ⇒ T)’
-    suffices_by rw []
-  \\ ho_match_mp_tac exp_rel_strongind \\ rw []
-  >~ [‘Value v’] >- (
-    dxrule_then assume_tac env_rel_OPTREL
-    \\ first_x_assum (qspec_then ‘n’ assume_tac)
-    \\ gvs [ALOOKUP_FILTER, OPTREL_def, ALOOKUP_NONE, MAP_REVERSE]
-    \\ simp [subst_def, exp_rel_def, ALOOKUP_APPEND]
-    \\ imp_res_tac ALOOKUP_SOME \\ gs [MAP_REVERSE]
-    \\ CASE_TAC \\ gs [ALOOKUP_SOME])
-  >~ [‘Lit _’] >-
-   (dxrule_then assume_tac env_rel_OPTREL
-    \\ first_x_assum (qspec_then ‘n’ assume_tac)
-    \\ gvs [ALOOKUP_FILTER, OPTREL_def, ALOOKUP_NONE, MAP_REVERSE]
-    \\ simp [subst_def, exp_rel_def, ALOOKUP_APPEND]
-    \\ imp_res_tac ALOOKUP_SOME \\ gs [MAP_REVERSE]
-    \\ CASE_TAC \\ gs [ALOOKUP_SOME])
-  >~ [‘Cons _ []’] >-
-   (dxrule_then assume_tac env_rel_OPTREL
-    \\ first_x_assum (qspec_then ‘n’ assume_tac)
-    \\ gvs [ALOOKUP_FILTER, OPTREL_def, ALOOKUP_NONE, MAP_REVERSE]
-    \\ simp [subst_def, exp_rel_def, ALOOKUP_APPEND]
-    \\ imp_res_tac ALOOKUP_SOME \\ gs [MAP_REVERSE]
-    \\ CASE_TAC \\ gs [ALOOKUP_SOME])
-  >~ [‘Var n’] >- (
-    dxrule_then assume_tac env_rel_OPTREL
-    \\ first_x_assum (qspec_then ‘n’ assume_tac)
-    \\ simp [subst_def]
-    \\ gvs [ALOOKUP_FILTER, OPTREL_def]
-    \\ (irule exp_rel_Var ORELSE irule exp_rel_Value)
-    \\ gs [ALOOKUP_APPEND, ALOOKUP_NONE, MAP_REVERSE])
-  >~ [‘App f x’] >- (
-    simp [subst_def, exp_rel_def])
-  >~ [‘Lam s x’] >- (
-    simp [subst_def, exp_rel_def, FILTER_APPEND_DISTRIB]
-    \\ first_x_assum irule
-    \\ gs [FILTER_FILTER, LAMBDA_PROD, MAP_FST_FILTER, env_rel_def,
-           GSYM FILTER_REVERSE]
-    \\ qabbrev_tac ‘P = λn. n ≠ s’ \\ gs []
-    \\ irule_at Any LIST_REL_FILTER
-    \\ irule_at Any env_rel_MAP_FST \\ gs [env_rel_def, Abbr ‘P’]
-    \\ gvs [LIST_REL_EL_EQN]
-    \\ irule_at Any LIST_EQ
-    \\ gvs [EL_MAP, ELIM_UNCURRY, MEM_FILTER]
-    \\ rw [DISJ_EQ_IMP, SF CONJ_ss, AC CONJ_COMM CONJ_ASSOC])
-  >~ [‘Seq x y’] >- (
-    simp [subst_def, exp_rel_def])
-  >~ [‘Let (SOME n) x y’] >- (
-    simp [subst_def, exp_rel_def, FILTER_APPEND_DISTRIB]
-    \\ first_x_assum irule
-    \\ gvs [FILTER_FILTER, LAMBDA_PROD, GSYM FST_THM, MAP_FST_FILTER,
-            MEM_FILTER]
-    \\ qabbrev_tac ‘P = λx. x ≠ n’ \\ gs []
-    \\ rw [DISJ_EQ_IMP, SF CONJ_ss, AC CONJ_COMM CONJ_ASSOC]
-    \\ gs [env_rel_def, GSYM FILTER_REVERSE]
-    \\ irule LIST_REL_FILTER
-    \\ gvs [LIST_REL_EL_EQN]
-    \\ irule LIST_EQ
-    \\ gvs [EL_MAP, ELIM_UNCURRY])
-  >~ [‘If x1 y1 z1’] >- (
-    simp [subst_def, exp_rel_def])
-  >~ [‘Prim op xs’] >- (
-    simp [subst_def, exp_rel_def, EVERY2_MAP, SF ETA_ss]
-    \\ gvs [LIST_REL_EL_EQN])
-  >~ [‘Letrec f x’] >- (
-    gs [subst_def, exp_rel_def, EVERY2_MAP, FILTER_FILTER, LAMBDA_PROD,
-        MAP_MAP_o, combinTheory.o_DEF, GSYM FST_THM, FILTER_APPEND_DISTRIB]
-    \\ first_x_assum (irule_at Any)
-    \\ qabbrev_tac ‘P = λn. ¬MEM n (MAP FST f)’ \\ gs []
-    \\ gs [MAP_FST_FILTER, MEM_FILTER, FILTER_FILTER, DISJ_EQ_IMP, LAMBDA_PROD]
-    \\ gs [SF CONJ_ss, AC CONJ_COMM CONJ_ASSOC, env_rel_def,
-           GSYM FILTER_REVERSE]
-    \\ irule_at Any LIST_REL_FILTER
-    \\ irule_at Any LIST_REL_mono
-    \\ first_assum (irule_at Any)
-    \\ simp [LAMBDA_PROD, FORALL_PROD]
-    \\ irule_at Any env_rel_MAP_FST \\ gvs [env_rel_def]
-    \\ simp [GSYM MAP_REVERSE, LIST_REL_MAP1, combinTheory.o_DEF, LAMBDA_PROD]
-    \\ irule LIST_REL_mono
-    \\ first_assum (irule_at Any)
-    \\ rw [FORALL_PROD] \\ gvs [ELIM_UNCURRY]
-    \\ first_x_assum (irule_at Any)
-    \\ simp [MAP_FST_FILTER, LAMBDA_PROD, MEM_FILTER, DISJ_EQ_IMP, SF CONJ_ss,
-             FILTER_FILTER, AC CONJ_COMM CONJ_ASSOC, GSYM FILTER_REVERSE]
-    \\ irule LIST_REL_FILTER
-    \\ irule_at Any env_rel_MAP_FST
-    \\ gvs [ELIM_UNCURRY, env_rel_def, LIST_REL_EL_EQN])
-  >~ [‘Delay x’] >- (
-    rw [subst_def, exp_rel_def])
-  >~ [‘Box x’] >- (
-    rw [subst_def, exp_rel_def])
-  >~ [‘Force x’] >- (
-    rw [subst_def, exp_rel_def])
-QED
-
-Theorem SUM_REL_def[local,simp] = quotient_sumTheory.SUM_REL_def;
-
-Theorem PAIR_REL_def[local,simp] = quotient_pairTheory.PAIR_REL;
-
-Theorem eval_to_exp_rel:
-  ∀k x env y.
-    exp_rel env x y ⇒
-      ($= +++ v_rel) (eval_to k x) (eval_to k env y)
-Proof
-  ho_match_mp_tac eval_to_ind \\ rw []
-  >~ [‘Value v’] >- (
-    gs [exp_rel_def, eval_to_def, envLangTheory.eval_to_def])
-  >~ [‘Var n’] >- (
-    gs [exp_rel_def, eval_to_def, envLangTheory.eval_to_def])
-  >~ [‘App f x’] >- (
-    gvs [exp_rel_def, eval_to_def, envLangTheory.eval_to_def]
-    \\ rename1 ‘exp_rel env f g’
-    \\ rename1 ‘exp_rel env x y’
-    \\ first_x_assum (drule_all_then assume_tac)
-    \\ first_x_assum (drule_all_then assume_tac)
-    \\ Cases_on ‘eval_to k x’ \\ Cases_on ‘eval_to k env y’ \\ gs []
-    \\ Cases_on ‘eval_to k f’ \\ Cases_on ‘eval_to k env g’ \\ gs []
-    \\ rename1 ‘v_rel v w’
-    \\ Cases_on ‘v’ \\ Cases_on ‘w’ \\ gvs [dest_anyClosure_def, v_rel_def,
-                                            envLangTheory.dest_anyClosure_def]
-    >- (
-      IF_CASES_TAC \\ gs []
-      \\ rename1 ‘v_rel v w’
-      \\ ‘[s,v] = [] ++ [s,v]’ by gs []
-      \\ pop_assum SUBST1_TAC
-      \\ first_x_assum (irule_at Any) \\ gs []
-      \\ ‘(s,w)::l = [s,w] ++ l’ by gs []
-      \\ pop_assum SUBST1_TAC
-      \\ irule exp_rel_subst
-      \\ gs [exp_rel_def, env_rel_def])
-    \\ qmatch_asmsub_abbrev_tac ‘LIST_REL (λ(a,x) (b,y). a = b ∧ R x y) xs ys’
-    \\ ‘OPTREL R (ALOOKUP xs s) (ALOOKUP ys s)’
-      by (‘xs = REVERSE (REVERSE xs)’ by gs [] \\ pop_assum SUBST1_TAC
-          \\ ‘ys = REVERSE (REVERSE ys)’ by gs [] \\ pop_assum SUBST1_TAC
-          \\ irule LIST_REL_OPTREL
-          \\ gvs [LIST_REL_EL_EQN])
-    \\ gs [OPTREL_def, Abbr ‘ys’, Abbr ‘R’]
-    \\ qpat_x_assum ‘exp_rel _ x0 y0’ mp_tac
-    \\ rw [Once exp_rel_cases] \\ gs []
-    \\ IF_CASES_TAC \\ gs []
-    \\ first_x_assum (irule_at Any)
-    \\ qmatch_goalsub_abbrev_tac ‘exp_rel (A::(B ++ C))’
-    \\ ‘A::(B ++ C) = A::B ++ C’ by gs []
-    \\ pop_assum SUBST1_TAC
-    \\ irule exp_rel_subst
-    \\ unabbrev_all_tac
-    \\ gs [MAP_MAP_o, combinTheory.o_DEF, LAMBDA_PROD, GSYM FST_THM,
-           FILTER_FILTER, AC CONJ_COMM CONJ_ASSOC]
-    \\ gs [env_rel_def, LIST_REL_EL_EQN, ELIM_UNCURRY, EL_MAP, EL_REVERSE,
-           v_rel_def])
-  >~ [‘Lam s x’] >- (
-    gvs [exp_rel_def, eval_to_def, envLangTheory.eval_to_def, v_rel_def])
-  >~ [‘Seq x1 y1’] >- (
-    gvs [exp_rel_def, eval_to_def, envLangTheory.eval_to_def, v_rel_def]
-    \\ IF_CASES_TAC \\ gs []
-    \\ last_x_assum (drule_all_then assume_tac)
-    \\ Cases_on ‘eval_to (k - 1) x1’
-    \\ Cases_on ‘eval_to (k - 1) env x2’ \\ gs [])
-  >~ [‘Let (SOME n) x1 y1’] >- (
-    gvs [exp_rel_def, eval_to_def, envLangTheory.eval_to_def, v_rel_def]
-    \\ IF_CASES_TAC \\ gs []
-    \\ last_x_assum (drule_all_then assume_tac)
-    \\ Cases_on ‘eval_to (k - 1) x1’
-    \\ Cases_on ‘eval_to (k - 1) env x2’ \\ gs []
-    \\ rename1 ‘v_rel v w’
-    \\ first_x_assum irule
-    \\ ‘(n,w)::env = [n,w] ++ env’ by gs []
-    \\ pop_assum SUBST_ALL_TAC
-    \\ irule exp_rel_subst
-    \\ gs [env_rel_def])
-  >~ [‘If x1 y1 z1’] >- (
-    gvs [exp_rel_def, eval_to_def, envLangTheory.eval_to_def, v_rel_def]
-    \\ IF_CASES_TAC \\ gs []
-    \\ first_x_assum (drule_all_then assume_tac)
-    \\ first_x_assum (drule_all_then assume_tac)
-    \\ first_x_assum (drule_all_then assume_tac)
-    \\ Cases_on ‘eval_to (k - 1) x1’
-    \\ Cases_on ‘eval_to (k - 1) env x2’ \\ gs []
-    \\ IF_CASES_TAC \\ gs [v_rel_def]
-    \\ IF_CASES_TAC \\ gs [v_rel_def]
-    \\ IF_CASES_TAC \\ gs [v_rel_def]
-    \\ IF_CASES_TAC \\ gs [v_rel_def])
-  >~ [‘Letrec f x’] >- (
-    gvs [exp_rel_def, eval_to_def, envLangTheory.eval_to_def, v_rel_def]
-    \\ IF_CASES_TAC \\ gs []
-    \\ first_x_assum irule
-    \\ simp [subst_funs_def]
-    \\ irule exp_rel_subst
-    \\ gvs [MAP_MAP_o, combinTheory.o_DEF, LAMBDA_PROD, GSYM FST_THM]
-    \\ gvs [env_rel_def, LIST_REL_EL_EQN, ELIM_UNCURRY, EL_MAP, EL_REVERSE,
-            v_rel_def])
-  >~ [‘Delay x’] >- (
-    gvs [exp_rel_def, eval_to_def, envLangTheory.eval_to_def, v_rel_def])
-  >~ [‘Box x’] >- (
-    gvs [exp_rel_def, eval_to_def, envLangTheory.eval_to_def, v_rel_def]
-    \\ first_x_assum (drule_all_then assume_tac)
-    \\ rename1 ‘exp_rel _ x y’
-    \\ Cases_on ‘eval_to k x’ \\ Cases_on ‘eval_to k env y’ \\ gs [v_rel_def])
-  >~ [‘Force x’] >- (
-    gvs [exp_rel_def]
-    \\ rename1 ‘exp_rel _ x y’
-    \\ simp [Once eval_to_def, envLangTheory.eval_to_def]
-    \\ IF_CASES_TAC \\ gs []
-    \\ first_x_assum (drule_all_then assume_tac)
-    \\ gs [PULL_EXISTS]
-    \\ Cases_on ‘eval_to k x’ \\ Cases_on ‘eval_to k env y’ \\ gs []
-    \\ rename1 ‘v_rel v w’
-    \\ reverse (Cases_on ‘dest_Tick v’) \\ gs []
-    >- (
-      Cases_on ‘v’ \\ gs []
-      \\ rgs [Once v_rel_cases])
-    \\ Cases_on ‘v’ \\ Cases_on ‘w’ \\ gvs [dest_anyThunk_def, v_rel_def,
-                                           envLangTheory.dest_anyThunk_def]
-    >- (
-      qmatch_asmsub_abbrev_tac
-        ‘LIST_REL (λ(a,x) (b,y). a = b ∧ R x y) xs ys’
-      \\ ‘OPTREL R (ALOOKUP xs s) (ALOOKUP ys s)’
-        by (‘xs = REVERSE (REVERSE xs)’ by gs [] \\ pop_assum SUBST1_TAC
-            \\ ‘ys = REVERSE (REVERSE ys)’ by gs [] \\ pop_assum SUBST1_TAC
-            \\ irule LIST_REL_OPTREL \\ gs [])
-      \\ gvs [OPTREL_def, Abbr ‘R’]
-      \\ pop_assum mp_tac
-      \\ rw [Once exp_rel_cases] \\ gs []
-      \\ first_x_assum irule
-      \\ gs [subst_funs_def]
-      \\ irule exp_rel_subst
-      \\ gs [MAP_MAP_o, combinTheory.o_DEF, LAMBDA_PROD, GSYM FST_THM]
-      \\ gvs [env_rel_def, LIST_REL_EL_EQN, ELIM_UNCURRY, EL_MAP, EL_REVERSE,
-              Abbr ‘xs’, v_rel_def])
-    \\ CASE_TAC \\ gvs [v_rel_def]
-    \\ first_x_assum irule
-    \\ simp [subst_funs_def])
-  >~ [‘MkTick x’] >- (
-    rgs [Once exp_rel_cases])
-  >~ [‘Prim op xs’] >- (
-    gvs [exp_rel_def, eval_to_def, envLangTheory.eval_to_def]
-    >- (fs [result_map_def] \\ simp [Once v_rel_cases])
-    >- (fs [result_map_def] \\ simp [Once v_rel_cases])
-    \\ Cases_on ‘op’ \\ gs []
-    >- ((* Cons *)
-      gvs [LIST_REL_EL_EQN, MEM_EL, PULL_EXISTS, SF ETA_ss]
-      \\ qmatch_goalsub_abbrev_tac ‘result_map f xs’
-      \\ qmatch_goalsub_abbrev_tac ‘result_map g ys’
-      \\ ‘($= +++ (LIST_REL v_rel)) (result_map f xs) (result_map g ys)’
-        suffices_by (
-          rw []
-          \\ Cases_on ‘result_map f xs’ \\ Cases_on ‘result_map g ys’ \\ gs []
-          \\ simp [v_rel_def])
-      \\ gs [result_map_def, MEM_EL, PULL_EXISTS, EL_MAP, SF CONJ_ss]
-      \\ unabbrev_all_tac
-      \\ IF_CASES_TAC \\ gs []
-      >- (
-        first_x_assum (drule_then assume_tac)
-        \\ first_x_assum (drule_all_then assume_tac)
-        \\ Cases_on ‘eval_to k env (EL n ys)’ \\ gvs [SF SFY_ss])
-      \\ gs [DECIDE “A ⇒ ¬(B < C) ⇔ B < C ⇒ ¬A”]
-      \\ IF_CASES_TAC \\ gs []
-      >- (
-        last_assum (drule_all_then assume_tac)
-        \\ last_assum (drule_all_then assume_tac)
-        \\ Cases_on ‘eval_to k env (EL n ys)’ \\ gvs [SF SFY_ss]
-        \\ IF_CASES_TAC \\ gs []
-        \\ rename1 ‘m < LENGTH ys’
-        \\ first_x_assum (drule_all_then assume_tac)
-        \\ first_x_assum (drule_all_then assume_tac)
-        \\ Cases_on ‘eval_to k (EL m xs)’ \\ gs [])
-      \\ gs [DECIDE “A ⇒ ¬(B < C) ⇔ B < C ⇒ ¬A”]
-      \\ IF_CASES_TAC \\ gs []
-      >- (
-        first_x_assum (drule_all_then assume_tac)
-        \\ first_x_assum (drule_all_then assume_tac)
-        \\ first_x_assum (drule_then assume_tac)
-        \\ first_x_assum (drule_then assume_tac)
-        \\ Cases_on ‘eval_to k (EL n xs)’ \\ gs [])
-      \\ gs [DECIDE “A ⇒ ¬(B < C) ⇔ B < C ⇒ ¬A”]
-      \\ IF_CASES_TAC \\ gs []
-      >- (
-        first_x_assum (drule_all_then assume_tac)
-        \\ first_x_assum (drule_all_then assume_tac)
-        \\ first_x_assum (drule_then assume_tac)
-        \\ first_x_assum (drule_then assume_tac)
-        \\ Cases_on ‘eval_to k (EL n xs)’ \\ gs [])
-      \\ gvs [DECIDE “A ⇒ ¬(B < C) ⇔ B < C ⇒ ¬A”, EVERY2_MAP, LIST_REL_EL_EQN]
-      \\ rw []
-      \\ first_x_assum (drule_all_then assume_tac)
-      \\ first_x_assum (drule_all_then assume_tac)
-      \\ rpt (first_x_assum (drule_then assume_tac))
-      \\ Cases_on ‘eval_to k (EL n xs)’
-      \\ Cases_on ‘eval_to k env (EL n ys)’ \\ gs []
-      \\ rename1 ‘INL err’ \\ Cases_on ‘err’ \\ gs [])
-    >- ((* IsEq *)
-      gvs [LIST_REL_EL_EQN]
-      \\ IF_CASES_TAC \\ gs []
-      \\ gvs [LENGTH_EQ_NUM_compute, DECIDE “∀n. n < 1 ⇔ n = 0”]
-      \\ IF_CASES_TAC \\ gs []
-      \\ rename1 ‘exp_rel env x y’
-      \\ first_x_assum (drule_then strip_assume_tac)
-      \\ Cases_on ‘eval_to (k - 1) x’
-      \\ Cases_on ‘eval_to (k - 1) env y’ \\ gs []
-      \\ rename1 ‘v_rel v w’
-      \\ Cases_on ‘v’ \\ Cases_on ‘w’ \\ gvs [v_rel_def]
-      \\ gvs [LIST_REL_EL_EQN]
-      \\ IF_CASES_TAC \\ gs [v_rel_def])
-    >- ((* Proj *)
-      gvs [LIST_REL_EL_EQN]
-      \\ IF_CASES_TAC \\ gs []
-      \\ gvs [LENGTH_EQ_NUM_compute, DECIDE “∀n. n < 1 ⇔ n = 0”]
-      \\ IF_CASES_TAC \\ gs []
-      \\ rename1 ‘exp_rel env x y’
-      \\ first_x_assum (drule_then strip_assume_tac)
-      \\ Cases_on ‘eval_to (k - 1) x’
-      \\ Cases_on ‘eval_to (k - 1) env y’ \\ gs []
-      \\ rename1 ‘v_rel v w’
-      \\ Cases_on ‘v’ \\ Cases_on ‘w’ \\ gvs [v_rel_def]
-      \\ gvs [LIST_REL_EL_EQN]
-      \\ IF_CASES_TAC \\ gs [v_rel_def])
-    >- ((* AtomOp *)
-      gvs [LIST_REL_EL_EQN, MEM_EL, PULL_EXISTS]
-      \\ Cases_on ‘k = 0’ \\ gs []
-      >- (
-        simp [result_map_def, MEM_MAP, GSYM NOT_NULL_MEM, NULL_EQ]
-        \\ rw [] \\ gvs []
-        \\ CASE_TAC \\ gs []
-        \\ CASE_TAC \\ gs [v_rel_def])
-      \\ qmatch_goalsub_abbrev_tac ‘result_map f xs’
-      \\ qmatch_goalsub_abbrev_tac ‘result_map g ys’
-      \\ ‘result_map f xs = result_map g ys’
-        suffices_by (
-          rw []
-          \\ Cases_on ‘result_map g ys’ \\ gs []
-          \\ CASE_TAC \\ gs []
-          \\ CASE_TAC \\ gs [v_rel_def])
-      \\ gs [result_map_def, MEM_EL, PULL_EXISTS, EL_MAP, SF CONJ_ss]
-      \\ unabbrev_all_tac
-      \\ IF_CASES_TAC \\ gs []
-      >- (
-        first_x_assum (drule_then assume_tac)
-        \\ first_x_assum (drule_all_then assume_tac)
-        \\ rw [] \\ gs [DECIDE “A ⇒ ¬(B < C) ⇔ B < C ⇒ ¬A”]
-        \\ rpt (first_x_assum (qspec_then ‘n’ assume_tac)) \\ gs []
-        \\ Cases_on ‘eval_to (k - 1) (EL n xs)’
-        \\ Cases_on ‘eval_to (k - 1) env (EL n ys)’ \\ gs []
-        \\ rename1 ‘v_rel v w’
-        \\ Cases_on ‘v’ \\ Cases_on ‘w’ \\ gs [v_rel_def])
-      \\ gs [DECIDE “A ⇒ ¬(B < C) ⇔ B < C ⇒ ¬A”]
-      \\ IF_CASES_TAC \\ gs []
-      >- (
-        rw [] \\ gs [DECIDE “A ⇒ ¬(B < C) ⇔ B < C ⇒ ¬A”]
-        >- (
-          rename1 ‘m < LENGTH ys’
-          \\ last_x_assum (drule_all_then assume_tac)
-          \\ last_x_assum (drule_all_then assume_tac)
-          \\ rpt (first_x_assum (qspec_then ‘m’ assume_tac)) \\ gs []
-          \\ Cases_on ‘eval_to (k - 1) (EL m xs)’
-          \\ Cases_on ‘eval_to (k - 1) env (EL m ys)’ \\ gs []
-          \\ rename1 ‘v_rel v w’
-          \\ Cases_on ‘v’ \\ Cases_on ‘w’ \\ gs [v_rel_def])
-        \\ last_x_assum (drule_all_then assume_tac)
-        \\ last_x_assum (drule_all_then assume_tac)
-        \\ rpt (first_x_assum (qspec_then ‘n’ assume_tac)) \\ gs []
-        \\ Cases_on ‘eval_to (k - 1) (EL n xs)’
-        \\ Cases_on ‘eval_to (k - 1) env (EL n ys)’ \\ gs []
-        \\ rename1 ‘v_rel v w’
-        \\ Cases_on ‘v’ \\ Cases_on ‘w’ \\ gs [v_rel_def])
-      \\ rw [] \\ gs [DECIDE “A ⇒ ¬(B < C) ⇔ B < C ⇒ ¬A”]
-      >- (
-        first_x_assum (drule_all_then assume_tac)
-        \\ first_x_assum (drule_all_then assume_tac)
-        \\ rpt (first_x_assum (drule_then assume_tac))
-        \\ Cases_on ‘eval_to (k - 1) (EL n xs)’
-        \\ Cases_on ‘eval_to (k - 1) env (EL n ys)’ \\ gs []
-        \\ rename1 ‘v_rel v w’
-        \\ Cases_on ‘v’ \\ Cases_on ‘w’ \\ gs [v_rel_def])
-      >- (
-        first_x_assum (drule_all_then assume_tac)
-        \\ first_x_assum (drule_all_then assume_tac)
-        \\ rpt (first_x_assum (drule_then assume_tac))
-        \\ Cases_on ‘eval_to (k - 1) (EL n xs)’
-        \\ Cases_on ‘eval_to (k - 1) env (EL n ys)’ \\ gs []
-        \\ rename1 ‘v_rel v w’
-        \\ Cases_on ‘v’ \\ Cases_on ‘w’ \\ gs [v_rel_def])
-      \\ irule LIST_EQ
-      \\ gs [MAP_MAP_o, combinTheory.o_DEF, EL_MAP]
-      \\ qx_gen_tac ‘m’ \\ rw []
-      \\ first_x_assum (drule_all_then assume_tac)
-      \\ first_x_assum (drule_all_then assume_tac)
-      \\ rpt (first_x_assum (drule_then assume_tac))
-      \\ Cases_on ‘eval_to (k - 1) (EL m xs)’
-      \\ Cases_on ‘eval_to (k - 1) env (EL m ys)’ \\ gs []
-      \\ rename1 ‘v_rel v w’
-      \\ Cases_on ‘v’ \\ Cases_on ‘w’ \\ gs [v_rel_def]))
-QED
-
-Theorem eval_exp_rel:
-  exp_rel env x y ⇒
-    ($= +++ v_rel) (eval x) (eval env y)
-Proof
-  rw [thunkLangTheory.eval_def, envLangTheory.eval_def]
-  \\ DEEP_INTRO_TAC some_intro
-  \\ DEEP_INTRO_TAC some_intro \\ simp []
-  \\ simp [PULL_FORALL]
-  \\ qx_gen_tac ‘i’
-  \\ qx_gen_tac ‘j’
-  \\ qx_gen_tac ‘k’
-  \\ rw [] \\ gs []
-  >- (
-    drule_all_then (qspec_then ‘i + j’ assume_tac) eval_to_exp_rel
-    \\ drule_then (qspec_then ‘i + j’ assume_tac) eval_to_mono
-    \\ drule_then (qspec_then ‘i + j’ assume_tac) envLangTheory.eval_to_mono
-    \\ gs [])
-  >- (
-    drule_all_then (qspec_then ‘i’ assume_tac) eval_to_exp_rel
-    \\ first_x_assum (qspec_then ‘i’ assume_tac) \\ gs [])
-  \\ drule_all_then (qspec_then ‘k’ assume_tac) eval_to_exp_rel
-  \\ first_x_assum (qspec_then ‘k’ assume_tac) \\ gs []
-QED
-
-(************************)
-
-Definition cont_rel_def[simp]:
-  cont_rel thunk_semantics$Done env_semantics$Done = T ∧
-  cont_rel (BC v c) (BC w d) = (v_rel v w ∧ cont_rel c d) ∧
-  cont_rel (HC v c) (HC w d) = (v_rel v w ∧ cont_rel c d) ∧
-  cont_rel _ _ = F
+Definition get_arg_def:
+  get_arg n [] = env_cexp$Prim (Cons (strlit "")) [] ∧
+  get_arg n (x::xs) = if n = 0:num then x else get_arg (n-1) xs
 End
 
-Definition next_rel_def[simp]:
-  next_rel (Act a c s) (env_semantics$Act b d t) =
-    (a = b ∧ cont_rel c d ∧ LIST_REL (LIST_REL v_rel) s t) ∧
-  next_rel Ret Ret = T ∧
-  next_rel Div Div = T ∧
-  next_rel Err Err = T ∧
-  next_rel (_: (string # string) thunk_semantics$next_res) _ = F
+Definition remove_Delay_def[simp]:
+  remove_Delay (env_cexp$Delay x) = x ∧
+  remove_Delay y = y
 End
 
-Triviality LIST_REL_ALOOKUP_lemma:
-  ∀f g s.
-    LIST_REL (λ(fn,b) (gn,c). fn = gn ∧ exp_rel xs b c) f g ⇒
-    ALOOKUP f s = NONE ∧ ALOOKUP g s = NONE ∨
-    ∃b c.
-      ALOOKUP f s = SOME b ∧
-      ALOOKUP g s = SOME c ∧ exp_rel xs b c
-Proof
-  Induct \\ fs [PULL_EXISTS,FORALL_PROD]
-  \\ rpt gen_tac \\ strip_tac
-  \\ IF_CASES_TAC \\ fs []
-QED
+Definition to_env_def:
+  to_env ((Var v):thunk_cexp$cexp) = Var v:env_cexp$cexp ∧
+  to_env (Let opt x y) = Let opt (to_env x) (to_env y) ∧
+  to_env (Lam vs x) = Lams vs (to_env x) ∧
+  to_env (App x xs) = Apps (to_env x) (MAP to_env xs) ∧
+  to_env (Delay x) = Delay (to_env x) ∧
+  to_env (Force x) = Force (to_env x) ∧
+  to_env (Box x) = Box (to_env x) ∧
+  to_env (Letrec fs x) = Letrec (REVERSE (MAP (λ(n,x). (n,to_env x)) fs)) (to_env x) ∧
+  to_env (Case v rows d) = Case (Var v) v (MAP (λ(n,p,x). (n,p,to_env x)) rows) ∧
+  to_env (Prim p xs) =
+    let ys = MAP to_env xs in
+      case p of
+      | AtomOp a => Prim (AtomOp a) ys
+      | Cons n =>
+          let y0 = get_arg 0 ys in
+          let x0 = remove_Delay (get_arg 0 ys) in
+          let x1 = remove_Delay (get_arg 1 ys) in
+          let x2 = remove_Delay (get_arg 2 ys) in
+            if n = strlit "Ret"    then Ret y0          else
+            if n = strlit "Raise"  then Raise y0        else
+            if n = strlit "Bind"   then Bind x0 x1      else
+            if n = strlit "Handle" then Handle x0 x1    else
+            if n = strlit "Act"    then Act x0          else
+            if n = strlit "Length" then Length x0       else
+            if n = strlit "Alloc"  then Alloc x0 x1     else
+            if n = strlit "Deref"  then Deref x0 x1     else
+            if n = strlit "Update" then Update x0 x1 x2 else
+              Prim (Cons n) ys
+Termination
+  WF_REL_TAC ‘measure cexp_size’
+End
 
-Theorem LIST_REL_MAP_MAP:
-  ∀xs ys f g.
-    LIST_REL P (MAP f xs) (MAP g ys) ⇔
-    LIST_REL (λx y. P (f x) (g y)) xs ys
+Theorem to_env_exp_of:
+  ∀x. cexp_wf x ⇒ exp_rel [] (exp_of x) (exp_of (to_env x))
 Proof
-  Induct \\ fs [PULL_EXISTS]
-  \\ rw [] \\ eq_tac \\ rw [] \\ fs []
-  \\ Cases_on ‘ys’ \\ gvs []
-QED
-
-Theorem force_thm:
-  ∀v w. v_rel v w ⇒ ($= +++ v_rel) (force v) (force w)
-Proof
-  fs [force_def,env_semanticsTheory.force_def]
-  \\ reverse Cases \\ simp [Once v_rel_cases]
-  \\ fs [PULL_EXISTS]
-  \\ fs [dest_anyThunk_def,envLangTheory.dest_anyThunk_def]
-  \\ rw [] \\ gvs []
-  >~ [‘subst_funs []’]
-  >- (fs [subst_funs_def] \\ imp_res_tac eval_exp_rel \\ fs [])
-  \\ drule LIST_REL_ALOOKUP_lemma
-  \\ disch_then $ qspec_then ‘s’ strip_assume_tac
-  \\ fs []
-  \\ pop_assum mp_tac
-  \\ simp [Once exp_rel_cases]
-  \\ strip_tac \\ gvs []
-  \\ fs [subst_funs_def]
-  \\ irule eval_exp_rel
-  \\ irule exp_rel_subst
-  \\ fs [MAP_MAP_o,combinTheory.o_DEF,LAMBDA_PROD]
-  \\ fs [MEM_MAP,FORALL_PROD]
-  \\ fs [env_rel_def]
-  \\ fs [GSYM MAP_REVERSE]
-  \\ simp [LIST_REL_MAP_MAP,LAMBDA_PROD]
-  \\ fs [LIST_REL_EL_EQN]
-  \\ imp_res_tac LIST_REL_LENGTH
-  \\ fs []
-  \\ rw [LAMBDA_PROD]
-  \\ rpt (pairarg_tac \\ fs [])
-  \\ gvs []
-  \\ first_assum drule
-  \\ asm_rewrite_tac []
-  \\ fs [] \\ rw []
-  \\ simp [Once v_rel_cases]
-  \\ fs [LIST_REL_EL_EQN,MEM_MAP,FORALL_PROD]
-QED
-
-Theorem apply_closure_thm:
-  ∀v1 w1 v2 w2 f g.
-    v_rel v1 w1 ∧
-    v_rel v2 w2 ∧
-    (∀x y. ($= +++ v_rel) x y ⇒ next_rel (f x) (g y)) ⇒
-    next_rel (apply_closure v1 v2 f)
-             (apply_closure w1 w2 g)
-Proof
-  fs [apply_closure_def,env_semanticsTheory.apply_closure_def]
-  \\ fs [dest_anyClosure_def,envLangTheory.dest_anyClosure_def]
-  \\ simp [Once v_rel_cases] \\ rw [] \\ gvs []
-  >-
-   (first_x_assum irule
-    \\ irule eval_exp_rel
-    \\ once_rewrite_tac [GSYM (EVAL “[x:'a] ++ xs”)]
-    \\ irule exp_rel_subst \\ fs []
-    \\ fs [env_rel_def]
+  ho_match_mp_tac to_env_ind \\ rw [cexp_wf_def] \\ fs []
+  >~ [‘Var’] >-
+   (fs [to_env_def]
+    \\ irule exp_rel_Var \\ fs [])
+  >~ [‘Let’] >-
+   (fs [to_env_def]
+    \\ Cases_on ‘opt’ \\ fs []
+    >- (irule exp_rel_Let_NONE \\ fs [])
+    \\ irule exp_rel_Let_SOME \\ fs [])
+  >~ [‘Lam’] >-
+   (last_x_assum mp_tac \\ fs [to_env_def]
+    \\ qid_spec_tac ‘vs’ \\ Induct
+    \\ fs [Lams_def] \\ rw [] \\ fs []
+    \\ irule exp_rel_Lam \\ fs [])
+  >~ [‘App’] >-
+   (fs [to_env_def]
+    \\ qpat_x_assum ‘EVERY _ _’ mp_tac
     \\ last_x_assum mp_tac
-    \\ simp [Once exp_rel_cases])
-  \\ drule LIST_REL_ALOOKUP_lemma
-  \\ disch_then $ qspec_then ‘n’ strip_assume_tac
-  \\ fs []
-  \\ pop_assum mp_tac
-  \\ simp [Once exp_rel_cases]
-  \\ strip_tac \\ gvs []
-  \\ first_assum irule
-  \\ irule eval_exp_rel
-  \\ rewrite_tac [APPEND |> CONJUNCT2 |> GSYM]
-  \\ irule exp_rel_subst
-  \\ simp [MAP_MAP_o,combinTheory.o_DEF,LAMBDA_PROD,FILTER_FILTER]
-  \\ fs [MEM_MAP,FORALL_PROD,FILTER_FILTER]
-  \\ reverse conj_tac
+    \\ last_x_assum mp_tac
+    \\ last_x_assum mp_tac
+    \\ qid_spec_tac ‘x’
+    \\ qid_spec_tac ‘xs’
+    \\ Induct
+    \\ fs [Apps_def] \\ rw [] \\ fs [SF DNF_ss]
+    \\ ‘cexp_wf (App x [h])’ by fs [cexp_wf_def]
+    \\ last_x_assum drule
+    \\ fs [to_env_def,Apps_def]
+    \\ disch_then irule
+    \\ irule exp_rel_App
+    \\ gs [])
+  >~ [‘Delay’] >-
+   (fs [to_env_def] \\ irule exp_rel_Delay \\ fs [cexp_wf_def])
+  >~ [‘Force’] >-
+   (fs [to_env_def] \\ irule exp_rel_Force \\ fs [cexp_wf_def])
+  >~ [‘Box’] >-
+   (fs [to_env_def] \\ irule exp_rel_Box \\ fs [cexp_wf_def])
+  >~ [‘Letrec’] >-
+   (fs [to_env_def] \\ irule exp_rel_Letrec \\ fs [cexp_wf_def]
+    \\ fs [GSYM MAP_REVERSE,MAP_MAP_o,combinTheory.o_DEF]
+    \\ fs [LIST_REL_MAP_MAP,LAMBDA_PROD]
+    \\ irule EVERY2_refl \\ fs [FORALL_PROD,SF SFY_ss,EVERY_MEM])
+  >~ [‘Case’] >- cheat (* envLang and stateLang need updating *)
+  \\ rename [‘Prim’]
+  \\ reverse (Cases_on ‘p’)
   >-
-   (pop_assum mp_tac
-    \\ match_mp_tac (METIS_PROVE [] “x = y ⇒ (x ⇒ y)”)
-    \\ rpt (AP_TERM_TAC ORELSE AP_THM_TAC)
-    \\ fs [FUN_EQ_THM,FORALL_PROD]
-    \\ rw [] \\ eq_tac \\ rw [])
-  \\ fs [env_rel_def]
-  \\ fs [GSYM MAP_REVERSE]
-  \\ simp [LIST_REL_MAP_MAP,LAMBDA_PROD]
-  \\ fs [LIST_REL_EL_EQN]
-  \\ imp_res_tac LIST_REL_LENGTH
-  \\ fs []
-  \\ rw [LAMBDA_PROD]
-  \\ rpt (pairarg_tac \\ fs [])
-  \\ gvs []
-  \\ first_assum drule
-  \\ asm_rewrite_tac []
-  \\ simp_tac std_ss []
-  \\ fs [] \\ rw []
-  \\ simp [Once v_rel_cases]
-  \\ fs [LIST_REL_EL_EQN,MEM_MAP,FORALL_PROD]
+   (fs [to_env_def]
+    \\ irule exp_rel_Prim
+    \\ last_x_assum mp_tac
+    \\ pop_assum mp_tac
+    \\ qid_spec_tac ‘xs’
+    \\ Induct \\ fs [])
+  \\ fs [to_env_def,SF ETA_ss]
+  \\ fs [args_ok_def]
+  \\ rw [] \\ fs [get_arg_def,to_env_def,SF DNF_ss]
+  \\ irule exp_rel_Prim \\ fs [] \\ gvs []
+  \\ Induct_on ‘xs’ \\ fs []
 QED
 
-Triviality v_rel_RetVal[simp]:
-  v_rel (Constructor "Ret" [Thunk (INR (Lit a))]) (RetVal (Atom a))
+Theorem to_env_semantics:
+  cexp_wf x ∧ closed (exp_of x) ⇒
+  itree_of (exp_of x) =
+  itree_of (exp_of (to_env x))
 Proof
-  simp [Once v_rel_cases]
-  \\ simp [Once v_rel_cases]
-  \\ simp [Once exp_rel_cases]
-QED
-
-Triviality force_similar:
-  ($= +++ v_rel) (force x) (force y) ⇒
-  (force y = INL Type_error ⇔ force x = INL Type_error) ∧
-  (force y = INL Diverge ⇔ force x = INL Diverge)
-Proof
-  Cases_on ‘force y’ \\ Cases_on ‘force x’ \\ gvs []
-QED
-
-Theorem LIST_REL_LUPDATE:
-  ∀xs ys x y n.
-    LIST_REL R xs ys ∧ R x y ⇒
-    LIST_REL R (LUPDATE x n xs) (LUPDATE y n ys)
-Proof
-  Induct \\ fs [PULL_EXISTS,LUPDATE_def] \\ rw []
-  \\ Cases_on ‘n’ \\ fs [LUPDATE_def]
-QED
-
-Theorem next_thm:
-  ∀k v c s w d t.
-    ($= +++ v_rel) v w ∧
-    cont_rel c d ∧
-    LIST_REL (LIST_REL v_rel) s t ⇒
-      next_rel (next k v c s) (next k w d t)
-Proof
-  ho_match_mp_tac next_ind \\ rw []
-  \\ Cases_on ‘v’ \\ Cases_on ‘w’ \\ gvs []
-  >- (
-    simp [next_def,env_semanticsTheory.next_def]
-    \\ CASE_TAC \\ gs [])
-  \\ rename1 ‘v_rel v w’
-  \\ Cases_on ‘(∃s x. v = Closure s x) ∨
-               (∃f n. v = Recclosure f n) ∨
-               (∃x. v = Thunk x) ∨
-               (∃x. v = Atom x)’
-  >- (
-    gvs [] \\ fs [Once v_rel_cases]
-    \\ res_tac \\ rgs []
-    >~ [‘Atom x’] >- (
-      Cases_on ‘w’ \\ res_tac \\ gs []
-      \\ simp [next_def,env_semanticsTheory.next_def])
-    \\ simp [next_def,env_semanticsTheory.next_def])
-  \\ Cases_on ‘∃x. v = DoTick x’
-  >- (gvs [] \\ fs [Once v_rel_cases])
-  \\  fs []
-  \\ ‘∃nm vs. v = Constructor nm vs’
-    by (Cases_on ‘v’ \\ gs [])
-  \\ gvs [v_rel_def]
-  \\ simp [Once next_def]
-  \\ simp [Once env_semanticsTheory.next_def]
-  \\ imp_res_tac LIST_REL_LENGTH \\ fs []
-  \\ Cases_on ‘nm = "Ret"’ \\ gvs [] >-
-   (IF_CASES_TAC \\ gs [] \\ gvs []
-    \\ gvs [LIST_REL_EL_EQN, LENGTH_EQ_NUM_compute, DECIDE “∀x. x < 1n ⇔ x = 0”]
-    \\ Cases_on ‘k = 0’ \\ gs []
-    >- (Cases_on ‘c’ \\ Cases_on ‘d’ \\ gs [])
-    \\ reverse (Cases_on ‘c’ \\ Cases_on ‘d’ \\ gs [])
-    >- (first_x_assum irule \\ gs []
-        \\ simp [Once v_rel_cases])
-    \\ simp [force_apply_closure_def,
-             env_semanticsTheory.force_apply_closure_def]
-    \\ rename1 ‘v_rel v w’
-    \\ ‘($= +++ v_rel) (force v) (force w)’ by (irule force_thm \\ fs [])
-    \\ Cases_on ‘force v’ \\ Cases_on ‘force w’ \\ gs []
-    >- (CASE_TAC \\ gs [])
-    \\ irule apply_closure_thm \\ fs [])
-  \\ Cases_on ‘nm = "Raise"’ \\ gvs [] >-
-   (IF_CASES_TAC \\ gs [] \\ gvs []
-    \\ gvs [LIST_REL_EL_EQN, LENGTH_EQ_NUM_compute, DECIDE “∀x. x < 1n ⇔ x = 0”]
-    \\ Cases_on ‘k = 0’ \\ gs []
-    >- (Cases_on ‘c’ \\ Cases_on ‘d’ \\ gs [])
-    \\ Cases_on ‘c’ \\ Cases_on ‘d’ \\ gs []
-    >- (first_x_assum irule \\ gs []
-        \\ simp [Once v_rel_cases])
-    \\ simp [force_apply_closure_def,
-             env_semanticsTheory.force_apply_closure_def]
-    \\ rename1 ‘v_rel v w’
-    \\ ‘($= +++ v_rel) (force v) (force w)’ by (irule force_thm \\ fs [])
-    \\ Cases_on ‘force v’ \\ Cases_on ‘force w’ \\ gs []
-    >- (CASE_TAC \\ gs [])
-    \\ irule apply_closure_thm \\ fs [])
-  \\ Cases_on ‘nm = "Bind"’ \\ gvs [] >-
-   (IF_CASES_TAC \\ gs [] \\ gvs []
-    \\ rgs [LIST_REL_EL_EQN, LENGTH_EQ_NUM_compute,
-            DECIDE “∀x. x < 2n ⇔ x = 0 ∨ x = 1”]
-    \\ rw [] \\ rgs [SF DNF_ss]
-    \\ rename1 ‘v_rel v w’
-    \\ ‘($= +++ v_rel) (force v) (force w)’ by (irule force_thm \\ fs [])
-    \\ simp [Once next_def])
-  \\ Cases_on ‘nm = "Handle"’ \\ gvs [] >-
-   (IF_CASES_TAC \\ gs []
-    \\ gs [] \\ res_tac \\ gvs []
-    \\ rgs [LIST_REL_EL_EQN, LENGTH_EQ_NUM_compute,
-            DECIDE “∀x. x < 2n ⇔ x = 0 ∨ x = 1”]
-    \\ rw [] \\ rgs [SF DNF_ss]
-    \\ rename1 ‘v_rel v w’
-    \\ ‘($= +++ v_rel) (force v) (force w)’ by (irule force_thm \\ fs [])
-    \\ simp [Once next_def])
-  \\ Cases_on ‘nm = "Act"’ \\ gvs [] >-
-   (IF_CASES_TAC \\ gs []
-    \\ gs [LIST_REL_EL_EQN, LENGTH_EQ_NUM_compute, DECIDE “∀x. x < 1n ⇔ x = 0”]
-    \\ simp [with_atoms_def, result_map_def, env_semanticsTheory.with_atoms_def] \\ gvs[]
-    \\ rename1 ‘v_rel v w’
-    \\ ‘($= +++ v_rel) (force v) (force w)’ by (irule force_thm \\ fs [])
-    \\ Cases_on ‘force v’ \\ Cases_on ‘force w’ \\ gs []
-    >- (Cases_on `x'` \\ gs [])
-    \\ gvs []
-    \\ rename1 ‘v_rel a b’
-    \\ qpat_x_assum ‘v_rel a b’ mp_tac
-    \\ simp [Once v_rel_cases] \\ strip_tac \\ gvs []
-    \\ gvs [get_atoms_def,env_semanticsTheory.get_atoms_def]
-    \\ CASE_TAC \\ gs []
-    \\ gs [LIST_REL_EL_EQN])
-  \\ Cases_on ‘nm = "Alloc"’ \\ gvs [] >-
-   (IF_CASES_TAC \\ gs []
-    \\ rgs [LENGTH_EQ_NUM_compute,
-            DECIDE “∀x. x < 2n ⇔ x = 0 ∨ x = 1”, SF DNF_ss]
-    \\ simp [with_atoms_def, result_map_def, env_semanticsTheory.with_atoms_def] \\ gvs[]
-    \\ rename1 ‘v_rel v w’
-    \\ ‘($= +++ v_rel) (force v) (force w)’ by (irule force_thm \\ fs [])
-    \\ Cases_on ‘force v’ \\ Cases_on ‘force w’ \\ gs []
-    >- (Cases_on `x'` \\ gs [])
-    \\ qpat_x_assum ‘v_rel a b’ mp_tac
-    \\ simp [Once v_rel_cases] \\ strip_tac \\ gvs []
-    \\ gvs [get_atoms_def,env_semanticsTheory.get_atoms_def]
-    \\ CASE_TAC \\ gs []
-    \\ CASE_TAC \\ gs []
-    \\ first_x_assum irule \\ gs []
-    \\ simp [PULL_EXISTS]
-    \\ qexists_tac ‘[Int i]’ \\ simp [LIST_REL_REPLICATE_same]
-    \\ imp_res_tac LIST_REL_LENGTH \\ fs [])
-  \\ Cases_on ‘nm = "Length"’ \\ gvs [] >-
-   (IF_CASES_TAC \\ gs []
-    \\ gs [] \\ res_tac \\ gvs []
-    \\ gs [LIST_REL_EL_EQN, LENGTH_EQ_NUM_compute, DECIDE “∀x. x < 1n ⇔ x = 0”]
-    \\ simp [with_atoms_def, result_map_def, env_semanticsTheory.with_atoms_def] \\ gvs[]
-    \\ rename1 ‘v_rel v w’
-    \\ ‘($= +++ v_rel) (force v) (force w)’ by (irule force_thm \\ fs [])
-    \\ Cases_on ‘force v’ \\ Cases_on ‘force w’ \\ gs []
-    >- (Cases_on `x'` \\ gs [])
-    \\ gvs []
-    \\ rename1 ‘v_rel a b’
-    \\ qpat_x_assum ‘v_rel a b’ mp_tac
-    \\ simp [Once v_rel_cases] \\ strip_tac \\ gvs []
-    \\ gvs [get_atoms_def,env_semanticsTheory.get_atoms_def]
-    \\ rpt (CASE_TAC \\ gs [])
-    \\ first_x_assum irule \\ gs []
-    \\ qexists_tac ‘[Loc n]’ \\ fs [])
-  \\ Cases_on ‘nm = "Deref"’ \\ gvs [] >-
-   (IF_CASES_TAC \\ gs []
-    \\ rgs [LENGTH_EQ_NUM_compute,
-            DECIDE “∀x. x < 2n ⇔ x = 0 ∨ x = 1”, SF DNF_ss]
-    \\ simp [with_atoms_def, result_map_def, env_semanticsTheory.with_atoms_def] \\ gvs[]
-    \\ rename [‘force h1 = INL Type_error ∨ force h2 = INL Type_error’]
-    \\ rename1 ‘v_rel h1' h1’
-    \\ rename1 ‘v_rel h2' h2’
-    \\ ‘($= +++ v_rel) (force h1') (force h1)’ by (irule force_thm \\ fs [])
-    \\ drule force_similar \\ strip_tac
-    \\ ‘($= +++ v_rel) (force h2') (force h2)’ by (irule force_thm \\ fs [])
-    \\ drule force_similar \\ strip_tac
-    \\ fs []
-    \\ IF_CASES_TAC \\ gvs []
-    \\ IF_CASES_TAC \\ gvs []
-    \\ Cases_on ‘force h1'’ \\ fs []
-    >- (Cases_on ‘x’ \\ gvs [])
-    \\ Cases_on ‘force h2'’ \\ fs []
-    >- (Cases_on ‘x’ \\ gvs [])
-    \\ Cases_on ‘force h1’ >- gvs []
-    \\ Cases_on ‘force h2’ >- gvs []
-    \\ gvs []
-    \\ qpat_x_assum ‘v_rel _ _’ mp_tac
-    \\ simp [Once v_rel_cases]
-    \\ qpat_x_assum ‘v_rel _ _’ mp_tac
-    \\ simp [Once v_rel_cases]
-    \\ rpt strip_tac \\ gvs []
-    \\ fs [thunk_semanticsTheory.get_atoms_def,
-           env_semanticsTheory.get_atoms_def]
-    \\ Cases_on ‘l’ \\ gvs []
-    \\ Cases_on ‘l'’ \\ gvs []
-    \\ imp_res_tac LIST_REL_LENGTH \\ gvs [] \\ fs []
-    \\ IF_CASES_TAC >- gvs []
-    \\ IF_CASES_TAC >- gvs []
-    \\ IF_CASES_TAC
-    >-
-     (fs [] \\ gvs [LIST_REL_EL_EQN]
-      \\ first_x_assum irule
-      \\ fs [PULL_EXISTS]
-      \\ qexists_tac ‘[Loc n; Int i]’ \\ fs []
-      \\ gvs [GSYM arithmeticTheory.NOT_LESS]
-      \\ simp [Once v_rel_cases]
-      \\ ‘Num i < LENGTH (EL n t)’ by (Cases_on ‘i’ \\ fs [])
-      \\ metis_tac [])
-    \\ ‘LENGTH (EL n t) = LENGTH (EL n s)’ by gvs [LIST_REL_EL_EQN]
-    \\ simp [] \\ gvs []
-    \\ first_x_assum $ qspec_then ‘[Loc n; Int i]’ mp_tac
-    \\ first_x_assum $ qspec_then ‘[Loc n; Int i]’ mp_tac
-    \\ first_x_assum $ qspec_then ‘[Loc n; Int i]’ mp_tac
-    \\ fs [] \\ rw []
-    >-
-     (first_x_assum irule \\ simp [PULL_EXISTS]
-      \\ simp [Once v_rel_cases]
-      \\ simp [Once v_rel_cases]
-      \\ simp [Once exp_rel_cases])
-    >-
-     (first_x_assum irule \\ simp [PULL_EXISTS]
-      \\ simp [Once v_rel_cases]
-      \\ simp [Once v_rel_cases]
-      \\ simp [Once exp_rel_cases]))
-  \\ Cases_on ‘nm = "Update"’ \\ gvs []
-  \\ IF_CASES_TAC \\ gs []
-  \\ gvs [LENGTH_EQ_NUM_compute]
-  \\ rename [‘next_rel (with_atoms [h1; h2] _) (with_atoms [h1'; h2'] _)’]
-  \\ ‘($= +++ v_rel) (force h1) (force h1')’ by (irule force_thm \\ fs [])
-  \\ drule force_similar \\ strip_tac
-  \\ ‘($= +++ v_rel) (force h2) (force h2')’ by (irule force_thm \\ fs [])
-  \\ drule force_similar \\ strip_tac
-  \\ simp [with_atoms_def, result_map_def, env_semanticsTheory.with_atoms_def]
-  \\ IF_CASES_TAC >- fs []
-  \\ IF_CASES_TAC >- fs []
-  \\ fs []
-  \\ Cases_on ‘force h1’ \\ fs []
-  \\ Cases_on ‘force h1'’ \\ gvs []
-  >- (Cases_on ‘x’ \\ gvs [])
-  \\ Cases_on ‘force h2’ \\ fs []
-  \\ Cases_on ‘force h2'’ \\ gvs []
-  >- (Cases_on ‘x’ \\ gvs [])
-  \\ qpat_x_assum ‘v_rel _ _’ mp_tac
-  \\ qpat_x_assum ‘v_rel _ _’ mp_tac
-  \\ simp_tac std_ss [Once v_rel_cases] \\ strip_tac
-  \\ gvs [get_atoms_def,env_semanticsTheory.get_atoms_def]
-  \\ simp_tac std_ss [Once v_rel_cases] \\ strip_tac
-  \\ gvs [get_atoms_def,env_semanticsTheory.get_atoms_def]
-  \\ Cases_on ‘l’ \\ fs []
-  \\ Cases_on ‘l'’ \\ fs []
-  \\ IF_CASES_TAC \\ fs []
-  \\ IF_CASES_TAC \\ fs []
-  \\ ‘LENGTH (EL n t) = LENGTH (EL n s)’ by gvs [LIST_REL_EL_EQN]
-  \\ simp []
-  \\ IF_CASES_TAC
-  >-
-   (gvs []
-    \\ first_x_assum irule
-    \\ fs [PULL_EXISTS]
-    \\ qexists_tac ‘[Loc n; Int i]’ \\ fs []
-    \\ simp [Once v_rel_cases]
-    \\ simp [Once v_rel_cases]
-    \\ irule_at Any LIST_REL_LUPDATE \\ fs []
-    \\ irule_at Any LIST_REL_LUPDATE \\ fs []
-    \\ conj_tac >- gvs [LIST_REL_EL_EQN]
-    \\ simp [Once exp_rel_cases])
-  \\ simp []
-  \\ first_x_assum irule \\ simp [PULL_EXISTS]
-  \\ qexists_tac ‘[Loc n; Int i]’ \\ fs []
-  \\ simp [Once v_rel_cases]
-  \\ simp [Once v_rel_cases]
-  \\ simp [Once exp_rel_cases]
-QED
-
-Theorem next_action_thm:
-  ($= +++ v_rel) v w ∧
-  cont_rel c d ∧
-  LIST_REL (LIST_REL v_rel) s t ⇒
-  next_rel (next_action v c s) (next_action w d t)
-Proof
-  strip_tac
-  \\ rw [next_action_def,env_semanticsTheory.next_action_def]
-  \\ DEEP_INTRO_TAC some_intro \\ simp []
-  \\ DEEP_INTRO_TAC some_intro \\ simp []
-  \\ simp [PULL_FORALL]
-  \\ qx_gen_tac ‘i’
-  \\ qx_gen_tac ‘j’
-  \\ qx_gen_tac ‘k’
-  \\ rw []
-  >-
-   (drule_all next_thm
-    \\ dxrule env_semanticsTheory.next_less_eq
-    \\ dxrule thunk_semanticsTheory.next_less_eq
-    \\ disch_then $ qspec_then ‘i+j’ assume_tac
-    \\ disch_then $ qspec_then ‘i+j’ assume_tac
-    \\ fs [])
-  >-
-   (last_x_assum (qspec_then ‘i’ assume_tac)
-    \\ drule_all_then assume_tac next_thm
-    \\ last_x_assum (qspec_then ‘i’ assume_tac)
-    \\ gvs [])
-  >-
-   (last_x_assum (qspec_then ‘k’ assume_tac)
-    \\ drule_all_then assume_tac next_thm
-    \\ last_x_assum (qspec_then ‘k’ assume_tac)
-    \\ gvs [])
-QED
-
-Theorem interp_eq:
-  ($= +++ v_rel) v w ∧
-  cont_rel c d ∧
-  LIST_REL (LIST_REL v_rel) s t ⇒
-  interp v c s = interp w d t
-Proof
-  strip_tac
-  \\ rw [Once itreeTheory.itree_bisimulation]
-  \\ qexists_tac `λt1 t2.
-    (t1 = t2 ∨
-     ∃v c s w d t.
-       interp v c s = t1 ∧
-       interp w d t = t2 ∧
-       ($= +++ v_rel) v w ∧
-       cont_rel c d ∧
-       LIST_REL (LIST_REL v_rel) s t)`
-  \\ rw []
-  >~ [‘interp v c s = interp w d t’] >-
-   (disj2_tac >> rpt $ irule_at Any EQ_REFL >> simp[])
-  \\ drule_all next_action_thm \\ strip_tac
-  \\ qpat_assum ‘interp _ _ _ = _’ mp_tac
-  >~ [‘Ret’] >-
-   (gvs []
-    \\ qpat_x_assum ‘thunk_semantics$interp _ _ _ = _’ mp_tac
-    \\ once_rewrite_tac [thunk_semanticsTheory.interp_def]
-    \\ once_rewrite_tac [env_semanticsTheory.interp_def]
-    \\ simp [AllCaseEqs()]
-    \\ rw [] \\ gvs []
-    \\ Cases_on `next_action w' d' t''` \\ gvs[])
-  >~ [‘Div’] >-
-   (gvs []
-    \\ qpat_x_assum ‘thunk_semantics$interp _ _ _ = _’ mp_tac
-    \\ once_rewrite_tac [thunk_semanticsTheory.interp_def]
-    \\ once_rewrite_tac [env_semanticsTheory.interp_def]
-    \\ simp [AllCaseEqs()]
-    \\ rw [] \\ gvs []
-    \\ Cases_on `next_action w' d' t''` \\ gvs[])
-  \\ gvs []
-  \\ qpat_x_assum ‘thunk_semantics$interp _ _ _ = _’ mp_tac
-  \\ simp [Once thunk_semanticsTheory.interp_def]
-  \\ simp [AllCaseEqs()]
-  \\ rw [] \\ gvs []
-  \\ Cases_on `next_action w' d' t''` \\ gvs[]
-  \\ simp [Once env_semanticsTheory.interp_def]
-  \\ rw []
-  \\ CASE_TAC \\ fs []
-  \\ CASE_TAC \\ fs []
-  \\ disj2_tac
-  \\ rpt (irule_at Any EQ_REFL)
-  \\ rpt $ first_assum $ irule_at Any
-  \\ fs []
-QED
-
-Theorem exp_rel_semantics:
-  exp_rel [] x y ∧
-  closed x ⇒
-  thunk_semantics$semantics x Done [] =
-  env_semantics$semantics y [] Done []
-Proof
-  strip_tac
-  \\ rw [thunk_semanticsTheory.semantics_def,env_semanticsTheory.semantics_def]
-  \\ irule interp_eq
-  \\ fs [state_rel_def]
-  \\ irule eval_exp_rel \\ fs []
+  rw [thunk_semanticsTheory.itree_of_def,env_semanticsTheory.itree_of_def]
+  \\ imp_res_tac to_env_exp_of
+  \\ drule_all exp_rel_semantics \\ fs []
 QED
 
 val _ = export_theory ();
